src/proof/iam_model/snapshot.v
@@ -1,0 +1,109 @@
+From New.proof Require Import prelude empty_ffi.
+From New.proof.iam_model Require Export common.
+From iris.algebra Require Import gmap gset.
+
+Section proof.
+Context `{hG: !heapGS Σ} `{!ffi_semantics _ _}.
+Context {sem : go.Semantics} {package_sem : iammodel.Assumptions}.
+Context `{!iamModelG Σ}.
+Local Set Default Proof Using "All".
+
+Lemma attachment_counts_dom_nonempty abs_identities policies resource :
+  dom (attachment_counts abs_identities policies resource) =
+  dom (filter (λ '(_, policy_ids),
+    attached_policies_for_resource policies policy_ids resource ≠ ∅)
+    abs_identities :
+    gmap iammodel.IdentityID.t (gmap iammodel.PolicyID.t unit)).
+Proof.
+  apply set_eq. intros identity.
+  rewrite !elem_of_dom. split.
+  - intros [n Hcount].
+    unfold attachment_counts, attachment_ref_counts,
+      counted_reversed_reference.reverse_index, attachment_state in Hcount.
+    rewrite !map_lookup_imap in Hcount.
+    destruct (abs_identities !! identity) as [policy_ids|] eqn:Hidentity;
+      simpl in Hcount; [|discriminate Hcount].
+    unfold counted_reversed_reference.reference_count in Hcount.
+    rewrite resource_count_refs_lookup in Hcount.
+    rewrite resources_for_identity_counts_lookup_default in Hcount.
+    destruct (decide
+      (0 < size (attached_policies_for_resource policies policy_ids resource))%nat)
+      as [Hpositive|Hnot_positive]; simpl in Hcount;
+      [|discriminate Hcount].
+    exists policy_ids. apply map_lookup_filter_Some. split; [done|].
+    intros Hempty. rewrite Hempty size_empty in Hpositive. lia.
+  - intros [policy_ids Hlookup].
+    apply map_lookup_filter_Some in Hlookup as [Hidentity Hnonempty].
+    exists (size (attached_policies_for_resource policies policy_ids resource)).
+    unfold attachment_counts, attachment_ref_counts,
+      counted_reversed_reference.reverse_index, attachment_state.
+    rewrite !map_lookup_imap Hidentity /=.
+    unfold counted_reversed_reference.reference_count.
+    rewrite resource_count_refs_lookup.
+    rewrite resources_for_identity_counts_lookup_default.
+    destruct (decide
+      (0 < size (attached_policies_for_resource policies policy_ids resource))%nat)
+      as [Hpositive|Hnot_positive]; simpl; [done|].
+    exfalso. apply Hnonempty.
+    apply leibniz_equiv, size_empty_inv. lia.
+Qed.
+
+Lemma wp_State__Snapshot γ l resource dq attachments :
+  {{{ "#Hiam" ∷ is_iam γ l ∗
+      "Hattachments" ∷ own_iam_attachments_frag γ resource dq attachments
+  }}}
+    l @! (go.PointerType iammodel.State) @! "Snapshot" #()
+  {{{ identities_l policies_l phys_identities abs_identities policies,
+      RET (#identities_l, #policies_l);
+      "Hattachments" ∷ own_iam_attachments_frag γ resource dq attachments ∗
+      "Hidentities" ∷ identities_l ↦$ phys_identities ∗
+      "Hidentities_inner" ∷ ([∗ map] policy_ids_l; policy_ids ∈
+        phys_identities; abs_identities, policy_ids_l ↦$ policy_ids) ∗
+      "Hpolicies" ∷ policies_l ↦$ policies ∗
+      "%Hattachments_consistent" ∷ ⌜
+        attachments = attachment_counts abs_identities policies resource ⌝ ∗
+      "%Hidentities_with_access" ∷ ⌜
+        dom attachments =
+        dom (filter (λ '(_, policy_ids),
+          attached_policies_for_resource policies policy_ids resource ≠ ∅)
+          abs_identities) ⌝
+  }}}.
+Proof.
+  iIntros (Φ) "(#Hiam & Hattachments) HΦ".
+  iDestruct "Hiam" as (mu_l) "[#Hmu #Hiam_inv]".
+  wp_method_call. rewrite /iammodel.State__Snapshotⁱᵐᵖˡ. wp_call.
+  wp_apply wp_with_defer as "%defer Hdefer". simpl subst. wp_auto.
+  wp_apply wp_Mutex__Lock;
+    [iFrame "#"; iEval (rewrite is_pkg_init_unfold /=);
+     iSplit; [iModIntro; iEval (rewrite !is_pkg_init_unfold /=); done|done]|].
+  iIntros "[Hown_Mutex H]". iNamedPrefix "H" "Hinv_". wp_auto.
+  iDestruct (own_attachments_frag_valid_pure with
+    "Hinv_Hown_attachments_auth Hattachments") as
+    %[Hattachments_consistent _].
+  rewrite exception_do_unseal /exception_do_def.
+  rewrite do_return_unseal.
+  wp_pures.
+  wp_apply (wp_copyIdentities with
+    "[$Hinv_Hown_phys_identities $Hinv_Hown_phys_identities_inner]").
+  iIntros (identities_l phys_identities_copy)
+    "(Hinv_Hown_phys_identities &
+      Hinv_Hown_phys_identities_inner & Hidentities & Hidentities_inner)".
+  wp_auto.
+  wp_apply (wp_copyPolicies with "[$Hinv_Hown_phys_policies]").
+  iIntros (policies_l) "[Hinv_Hown_phys_policies Hpolicies]".
+  iCombineNamed "Hinv_*" as "H".
+  wp_auto.
+  rewrite /exception.do_return_def.
+  wp_auto.
+  wp_apply (wp_Mutex__Unlock _ (iam_inv γ l) with "[$Hown_Mutex H]").
+  { iNamed "H". iFrame. iFrame "#%".
+    iEval (rewrite is_pkg_init_unfold /=).
+    iSplit; [iModIntro; iEval (rewrite !is_pkg_init_unfold /=); done|done]. }
+  iApply "HΦ". iFrame.
+  iPureIntro. split.
+  - done.
+  - rewrite Hattachments_consistent.
+    apply attachment_counts_dom_nonempty.
+Qed.
+
+End proof.
